user 3, session 10289, part 8

diffs-no-failures-no-compiles-clean/3/user-3-session-10289.v
@@ -5,51 +5,21 @@ Add Search Blacklist "Private_" "_subproof".
 Set Printing Depth 50.
 Remove Search Blacklist "Private_" "_subproof".
 Add Search Blacklist "Private_" "_subproof".
-Require Coq.Strings.String.
-Redirect "/var/folders/5x/1mdbpbjd7012l971fq0zkj2w0000gn/T/coq6EHQSi"
+Require Import Coq.Strings.String.
+Import StringSyntax.
+Redirect "/var/folders/5x/1mdbpbjd7012l971fq0zkj2w0000gn/T/coqrFgtUU"
 Print Ltac Signatures.
 Timeout 1 Print Grammar tactic.
 Add Search Blacklist "Raw" "Proofs".
 Set Search Output Name Only.
-Redirect "/var/folders/5x/1mdbpbjd7012l971fq0zkj2w0000gn/T/coqoeGQqP"
-SearchPattern _.
-Remove Search Blacklist "Raw" "Proofs".
-Unset Search Output Name Only.
-Timeout 1 Print LoadPath.
-Import Coq.Strings.String.StringSyntax.
-Redirect "/var/folders/5x/1mdbpbjd7012l971fq0zkj2w0000gn/T/coqk16bqe"
-Print Ltac Signatures.
-Timeout 1 Print Grammar tactic.
-Add Search Blacklist "Raw" "Proofs".
-Set Search Output Name Only.
-Redirect "/var/folders/5x/1mdbpbjd7012l971fq0zkj2w0000gn/T/coq77Gl8C"
+Redirect "/var/folders/5x/1mdbpbjd7012l971fq0zkj2w0000gn/T/coqIuiiUa"
 SearchPattern _.
 Remove Search Blacklist "Raw" "Proofs".
 Unset Search Output Name Only.
 Timeout 1 Print LoadPath.
 Require Import Helpers.Helpers.
-Redirect "/var/folders/5x/1mdbpbjd7012l971fq0zkj2w0000gn/T/coqzcx1u8"
-Print Ltac Signatures.
-Timeout 1 Print Grammar tactic.
-Add Search Blacklist "Raw" "Proofs".
-Set Search Output Name Only.
-Redirect "/var/folders/5x/1mdbpbjd7012l971fq0zkj2w0000gn/T/coqO6RHU6"
-SearchPattern _.
-Remove Search Blacklist "Raw" "Proofs".
-Unset Search Output Name Only.
-Timeout 1 Print LoadPath.
 Require Import Proc.
 Require Import ProcTheorems.
-Redirect "/var/folders/5x/1mdbpbjd7012l971fq0zkj2w0000gn/T/coq4DEKPQ"
-Print Ltac Signatures.
-Timeout 1 Print Grammar tactic.
-Add Search Blacklist "Raw" "Proofs".
-Set Search Output Name Only.
-Redirect "/var/folders/5x/1mdbpbjd7012l971fq0zkj2w0000gn/T/coq8Qd0ER"
-SearchPattern _.
-Remove Search Blacklist "Raw" "Proofs".
-Unset Search Output Name Only.
-Timeout 1 Print LoadPath.
 Record LayerAbstraction State1 State2 :={abstraction :
                                           State1 -> State2 -> Prop}.
 Definition Abstraction State := LayerAbstraction world State.
@@ -103,5 +73,38 @@ Proof.
 (destruct r; simpl in *; repeat deex; intuition eauto).
 Qed.
 Hint Resolve tt: core.
-Inductive Marker : string -> Type :=
+Inductive Marker : String.string -> Type :=
     mark : forall s, Marker s.
+Theorem proc_spec_rx :
+  forall `(spec : Specification A T R State) `(p : proc T) 
+    `(rec : proc R) `(rx : T -> proc T')
+    `(spec' : Specification A' T' R State) `(abs : Abstraction State),
+  proc_spec spec p rec abs ->
+  (forall a' state,
+   pre (spec' a' state) ->
+   exists a,
+     pre (spec a state) /\
+     (forall r state',
+      recovered (spec a state) r state' ->
+      Marker "recovered condition" -> recovered (spec' a' state) r state') /\
+     (forall r,
+      Marker "post condition" ->
+      proc_spec
+        (fun (_ : unit) state' =>
+         {|
+         pre := post (spec a state) r state';
+         post := fun r state'' => post (spec' a' state) r state'';
+         recovered := fun r state'' => recovered (spec' a' state) r state'' |})
+        (rx r) rec abs)) -> proc_spec spec' (Bind p rx) rec abs.
+Redirect "/var/folders/5x/1mdbpbjd7012l971fq0zkj2w0000gn/T/coqAYn5wi"
+Print Ltac Signatures.
+Timeout 1 Print Grammar tactic.
+Add Search Blacklist "Raw" "Proofs".
+Set Search Output Name Only.
+Redirect "/var/folders/5x/1mdbpbjd7012l971fq0zkj2w0000gn/T/coq7GSvsZ"
+SearchPattern _.
+Remove Search Blacklist "Raw" "Proofs".
+Unset Search Output Name Only.
+Timeout 1 Print LoadPath.
+Proof.
+(unfold proc_spec at 3; intros).
